\begin{problem}[Lagrange interpolant]
 
 Given data points $(t_i, y_i)_{i = 1}^n$, show that the Lagrange interpolant
 \[
  p(x) = \sum_{i = 0}^n y_i L_i(x), \quad L_i(x) := \prod_{\substack{j = 0\\ j \neq i}}^n \frac{x - t_j}{t_i - t_j}
 \]

 is given by:
 \[
  p(x) =  \omega(x)  \sum_{j = 0}^n \frac{y_j}{(x-t_j) \omega' (t_j)}
 \]
 with $\omega(x) = \prod_{j = 0}^n (x - t_j)$.
 
 \begin{solution}
 Simply exploiting the chain rule of many terms:
  \[
   \omega'(x) = \sum_{i = 0}^n \prod_{\substack{j = 0\\ j \neq i}}^n (x - t_j)
  \]
  Since $(t_i - t_j) = \delta_{i,j}$, it follows $\omega'(t_i) = \prod_{\substack{j = 0\\ j \neq i}}^n (t_i - t_j)$.
  Therefore:
  \begin{align*}
  p(x) =  \omega(x)  \sum_{j = 0}^n \frac{y_j}{(x-t_j) \omega' (t_j)} = \sum_{j = 0}^n \frac{y_j}{(x-t_j) \prod_{\substack{j = 0\\ j \neq i}}^n (t_i - t_j)} \prod_{j = 0}^n (x - t_j) \\
= \sum_{j = 0}^n \frac{y_j}{\prod_{\substack{j = 0\\ j \neq i}}^n (t_i - t_j)} \prod_{\substack{j = 0\\ j \neq i}}^n (x - t_j) = \sum_{j = 0}^n y_j \prod_{\substack{j = 0\\ j \neq i}}^n \frac{x - t_j}{t_i - t_j}.
  \end{align*}


 \end{solution}

 
\end{problem}
